adjusted clength to use Racket-generated constants

rkt/clength.rkt
@@ -1,0 +1,12 @@
+#lang at-exp s-exp "tmonad.rkt"
+
+(Fixpoint
+ clength #:implicit @A{Set} @l{list A}
+ #:returns @{nat}
+ (match (l)
+   [(nil) => (<== 0)]
+   [(cons a′ l′)
+    => 
+    (bind ((n′ (clength l′)))
+          (<== (+ n′ 1)))]))
+
